

# Generalized Linear Recursive Function for Complex Numbers

## 1 Definition of the Problem

We can define a generalized linear recursive function as one that follows:

$$f(n+1) = \sum_{j=0}^m a_j f(n-j) \quad (1)$$

where  $a_j$  are the coefficients of the function.

We will see how can we generalize this function to complex numbers as:

$$f(n) = \sum_{i=0}^{r-1} \sum_{k=0}^{d_i-1} c_{i,k} \lambda_i^{n-k} \prod_{j=0}^{k-1} (n-j) \quad (2)$$

where:

- $c_{i,k}$  are the coefficients of the function.
- $\lambda_i$  are the eigenvalues of the matrix  $A$ .
- $d_i$  is the multiplicity of the eigenvalue  $\lambda_i$ .
- $r$  is the number of distinct eigenvalues of the matrix  $A$ .
- $n \in \mathbb{C}$ .

This function is exactly the same as:

$$f(n) = \sum_{i=0}^{r-1} \lambda_i^n \sum_{k=0}^{d_i-1} c'_{i,k} n^k \quad (3)$$

Now the coefficients  $c'_{i,k}$  have a different meaning than  $c_{i,k}$  in previous formula

## 2 Summary of the Proof

We can rewrite the recursive function as:

$$\begin{pmatrix} f(n+1) \\ f(n) \\ f(n-1) \\ \vdots \\ f(n-m+3) \\ f(n-m+2) \\ f(n-m+1) \end{pmatrix} = \begin{pmatrix} a_0 & a_1 & a_2 & \cdots & a_{m-2} & a_{m-1} & a_m \\ 1 & 0 & 0 & \cdots & 0 & 0 & 0 \\ 0 & 1 & 0 & \cdots & 0 & 0 & 0 \\ \vdots & \vdots & \ddots & \ddots & \vdots & \vdots & \vdots \\ 0 & 0 & 0 & \cdots & 0 & 0 & 0 \\ 0 & 0 & 0 & \cdots & 1 & 0 & 0 \\ 0 & 0 & 0 & \cdots & 0 & 1 & 0 \end{pmatrix} \begin{pmatrix} f(n) \\ f(n-1) \\ f(n-2) \\ \vdots \\ f(n-m+2) \\ f(n-m+1) \\ f(n-m) \end{pmatrix} \quad (4)$$

If we have an initial conditions vector like,

$$F_0 = \begin{pmatrix} f(m) \\ f(m-1) \\ \vdots \\ f(1) \\ f(0) \end{pmatrix} \quad (5)$$

Therefore we can obtain  $F_n$  by just applying the operator A, n times to this vector.

$$F_n = A^n F_0 = \begin{pmatrix} f(n+m) \\ f(n+m-1) \\ \vdots \\ f(n+1) \\ f(n) \end{pmatrix} \quad (6)$$

We must obtain the eigenvalues and eigenvectors associated with matrix A.

$$P(\lambda) = \det(A - \lambda I) = 0 \quad (7)$$

which satisfy the following equation:

$$\lambda_i^{m+1} = \sum_{j=0}^m a_j \lambda_i^{m-j} \quad (8)$$

Each  $\lambda_i$  has only one associated eigenvector  $V_{i,0}$ ,

$$V_{i,0} = \begin{pmatrix} \lambda_i^m \\ \lambda_i^{m-1} \\ \vdots \\ \lambda_i \\ 1 \end{pmatrix} \quad (9)$$

If the number of distinct eigenvalues,  $r = m + 1$ . The problem is solved, we can express  $F_0$  as a linear combination of the eigenvectors  $V_{i,0}$ , because,

$$B = (V_{0,0}, V_{1,0}, \cdots, V_{m,0}) \text{ is a basis of } R^{m+1} \quad (10)$$

We proceed as follows:

- We express  $F_0$  as a linear combination of eigenvectors  $V_{i,0}$  that solve the corresponding system of equations, solving for the coefficients  $c_i$ .

$$F_0 = \sum_{i=0}^m c_i V_{i,0} \quad (11)$$

- We apply n times matrix A to  $F_0$  to obtain  $F_n$ .

$$F_n = A^n F_0 = \sum_{i=0}^m c_i A^n V_{i,0} \quad (12)$$

- Since  $A^n V_{i,0} = \lambda_i^n V_{i,0}$

$$F_n = \sum_{i=0}^m c_i \lambda_i^n V_{i,0} \quad (13)$$

- Our interest is on  $f_n$  which is the last term of the  $F_n$  vector, since all last terms of the vectors,  $V_{i,0}|_m = 1$ , we can write:

$$f(n) = \sum_{i=0}^m c_i \lambda_i^n \quad n \in \mathbb{C}. \quad (14)$$

Now imagine that some of our eigenvalues have degeneracy, because of this we cannot fill the space  $R^{m+1}$  with just the eigenvectors. For all eigenvalues with  $d_i > 1$  we will need to build  $d_i - 1$  additional vectors.

$$V_{i,k} = \left. \frac{d^k}{d\lambda^k} V_{i,0}(\lambda) \right|_{\lambda=\lambda_i} \quad k = 0, 1, \dots, d_i - 1. \quad (15)$$

Only  $V_{i,0}$  is an eigenvector.

An interesting property of these vectors is that when matrix A is applied to them, they behave as follows.

$$A V_{i,k} = k V_{i,k-1} + \lambda_i V_{i,k} \quad (16)$$

One shows by induction that

$$A^n V_{i,k} = \sum_{j=0}^{\min(n,k)} j! \binom{n}{j} \binom{k}{j} \lambda_i^{n-j} V_{i,k-j} \quad (17)$$

Since we know how  $A^n$  behaves when being applied to  $V_{i,k}$  we just need to follow the previous steps to get our generalized formula:

### 3 Interesting Properties

During the demonstration, the following identities appeared:

1. **Vandermonde's identity:**

$$\binom{n+m}{k} = \sum_{j=0}^k \binom{n}{j} \binom{m}{k-j}.$$

2. **Shifted polynomial identity:**

$$P_n(x) = \sum_{j=0}^n \binom{n}{j} (-1)^{j+1} P_n(x-j).$$

3. **Nested summations:** (creo que no la tengo demostrada)

$$\sum_{i_{n-1}=0}^{i_n-1} \sum_{i_{n-2}=0}^{i_{n-1}-1} \cdots \sum_{i_1=0}^{i_2-1} \sum_{i_0=0}^{i_1-1} 1 = \binom{i_n}{n}.$$

### 4 Calculation of the Eigenvalues

To calculate the eigenvalues,

$$\det(A - \lambda I) = \det(B) = 0 \quad (18)$$

We can write the elements  $B_{ij}$  like this,

$$B_{ij} = -\lambda \delta_{ij} + \delta_{ij+1} + a_j \delta_{i0} \quad (19)$$

We start by multiplying every column by  $\lambda^{m-j}$

$$B'_{ij} = B_{ij} \lambda^{m-j} = -\lambda^{m-j+1} \delta_{ij} + \lambda^{m-j} \delta_{ij+1} + \lambda^{m-j} a_j \delta_{i0} \quad (20)$$

$$\det(B') = \det(B) \lambda^{\frac{(m+1)m}{2}} \quad (21)$$

Then,

$$B''_{ij} = \sum_{k=j}^m B'_{ik} = -\lambda^{m-j+1} \delta_{ij} + \sum_{k=j}^m a_k \lambda^{m-k} \delta_{i0} \quad (22)$$

$$\det(B'') = \det(B') = \det(B) \lambda^{\frac{(m+1)m}{2}} \quad (23)$$

Then,

$$B'''_{ij} = B''_{ij} \lambda^{j-m} = -\lambda \delta_{ij} + \sum_{k=j}^m a_k \lambda^{j-k} \delta_{i0} \quad (24)$$

$$\det(B''') = \det(B'') \lambda^{\frac{-(m+1)m}{2}} = \det(B') \lambda^{\frac{-(m+1)m}{2}} = \det(B) \quad (25)$$

We can observe that  $B'''$  is triangular, because of that we can write the determinant like this,

$$\det(B''') = \det(B) = \prod_{i=0}^m B_{ii} = (-\lambda + \sum_{k=0}^m a_k \lambda^{-k}) \lambda^m \quad (26)$$

This is the equation that gives us the eigenvalues

$$\sum_{k=0}^m a_k \lambda^{m-k} = \lambda^{m+1} \quad (27)$$